theories/iris_opsem.v
@@ -166,7 +166,7 @@ Inductive pure_reduce : host_state -> store_record -> list host_value -> host_ex
            what we know to be non-existent.
 
          Also, the error message from the Lookup typeclass doesn't point to a specific line.. *)
-      hs !! id = Some (Some hv) ->
+      hs !! id = Some hv ->
       pure_reduce hs s locs (HE_getglobal id) hs s locs (HE_value hv)
   | pr_getglobal_trap:
     forall hs s locs id,
@@ -175,7 +175,7 @@ Inductive pure_reduce : host_state -> store_record -> list host_value -> host_ex
   | pr_setglobal_value:
     forall hs s locs id hv hs',
       hv <> HV_trap ->
-      hs' = <[id := Some hv]> hs ->
+      hs' = <[id := hv]> hs ->
       pure_reduce hs s locs (HE_setglobal id (HE_value hv)) hs' s locs (HE_value hv)
   | pr_setglobal_trap:
     forall hs s locs id,
@@ -194,7 +194,7 @@ Inductive pure_reduce : host_state -> store_record -> list host_value -> host_ex
       pure_reduce hs s locs (HE_getlocal n) hs s locs (HE_value HV_trap)
   | pr_setlocal:
     forall hs s locs n id locs' hv,
-      hs !! id = Some (Some hv) ->
+      hs !! id = Some hv ->
       (nat_of_N n) < length locs ->
       locs' = list_insert (N.to_nat n) hv locs ->
       pure_reduce hs s locs (HE_setlocal n id) hs s locs' (HE_value hv)
@@ -204,29 +204,25 @@ Inductive pure_reduce : host_state -> store_record -> list host_value -> host_ex
       pure_reduce hs s locs (HE_setlocal n id) hs s locs (HE_value HV_trap)
   | pr_setlocal_trap2:
     forall hs s locs n id hv,
-      hs !! id = Some (Some hv) ->
+      hs !! id = Some hv ->
       (nat_of_N n) >= length locs ->
       pure_reduce hs s locs (HE_setlocal n id) hs s locs (HE_value HV_trap)
   | pr_if_true:
     forall hs s locs id e1 e2 hv,
-      hs !! id = Some (Some hv) ->
+      hs !! id = Some hv ->
       hv <> HV_wasm_value (VAL_int32 (Wasm_int.int_zero i32m)) ->
       hv ≠ HV_trap ->
       pure_reduce hs s locs (HE_if id e1 e2) hs s locs e1
   | pr_if_false: 
     forall hs s locs id e1 e2 hv,
-      hs !! id = Some (Some hv) ->
+      hs !! id = Some hv ->
       hv = HV_wasm_value (VAL_int32 (Wasm_int.int_zero i32m)) ->
       pure_reduce hs s locs (HE_if id e1 e2) hs s locs e2
   | pr_if_trap: 
     forall hs s locs id e1 e2 hv,
-      hs !! id = Some (Some hv) ->
+      hs !! id = Some hv ->
       hv = HV_trap ->
       pure_reduce hs s locs (HE_if id e1 e2) hs s locs (HE_value HV_trap)
-  | pr_if_some_none: 
-    forall hs s locs id e1 e2,
-      hs !! id = Some None ->
-      pure_reduce hs s locs (HE_if id e1 e2) hs s locs e2
   | pr_if_none: 
     forall hs s locs id e1 e2,
       hs !! id = None ->
@@ -237,7 +233,7 @@ Inductive pure_reduce : host_state -> store_record -> list host_value -> host_ex
   (* record exprs *)
   | pr_new_rec:
     forall hs s locs kip hvs kvp,
-      list_extra.those2 (map (fun id => hs !! id) (unzip2 kip)) = Some hvs ->
+      list_extra.those (map (fun id => hs !! id) (unzip2 kip)) = Some hvs ->
       zip (unzip1 kip) hvs = kvp ->
       pure_reduce hs s locs (HE_new_rec kip) hs s locs (HE_value (HV_record kvp))
   | pr_new_rec_trap:
@@ -246,17 +242,17 @@ Inductive pure_reduce : host_state -> store_record -> list host_value -> host_ex
       pure_reduce hs s locs (HE_new_rec kip) hs s locs (HE_value HV_trap)
   | pr_getfield:
     forall hs s locs id fname kvp hv,
-      hs !! id = Some (Some (HV_record kvp)) ->
+      hs !! id = Some (HV_record kvp) ->
       lookup_kvp kvp fname = Some hv -> 
       pure_reduce hs s locs (HE_get_field id fname) hs s locs (HE_value hv)
   | pr_getfield_trap1:
     forall hs s locs id fname kvp,
-      hs !! id = Some (Some (HV_record kvp)) ->
+      hs !! id = Some (HV_record kvp) ->
       lookup_kvp kvp fname = None ->
       pure_reduce hs s locs (HE_get_field id fname) hs s locs (HE_value HV_trap)
   | pr_getfield_trap2:
     forall hs s locs id fname hv,
-      hs !! id = Some (Some hv) ->
+      hs !! id = Some hv ->
       host_typeof hv <> Some HT_record ->
       pure_reduce hs s locs (HE_get_field id fname) hs s locs (HE_value HV_trap)
   | pr_getfield_trap3:
@@ -271,11 +267,11 @@ Inductive pure_reduce : host_state -> store_record -> list host_value -> host_ex
       pure_reduce hs s locs (HE_new_host_func htf (N_of_nat locsn) e) hs s' locs (HE_value (HV_wov (WOV_funcref (Mk_funcidx n))))
   | pr_call_wasm:
     forall hs s ids cl id i j vts bes tf vs tn tm vars locs,
-      hs !! id = Some (Some (HV_wov (WOV_funcref (Mk_funcidx i)))) ->
+      hs !! id = Some (HV_wov (WOV_funcref (Mk_funcidx i))) ->
       s.(s_funcs) !! i = Some cl ->
       cl = FC_func_native j tf vts bes ->
       tf = Tf tn tm ->
-      list_extra.those2 (map (fun id => hs !! id) ids) = Some vars ->
+      list_extra.those (map (fun id => hs !! id) ids) = Some vars ->
       list_host_value_to_wasm vars = Some vs ->
       tn = map typeof vs ->
       pure_reduce hs s locs (HE_call id ids) hs s locs (HE_wasm_frame ((v_to_e_list vs) ++ [::AI_invoke i]))
@@ -285,44 +281,44 @@ Inductive pure_reduce : host_state -> store_record -> list host_value -> host_ex
       pure_reduce hs s locs (HE_call id ids) hs s locs (HE_value HV_trap)
   | pr_call_trap2:
     forall hs s locs id ids v,
-      hs !! id = Some (Some v) ->
+      hs !! id = Some v ->
       is_funcref v = false ->
       pure_reduce hs s locs (HE_call id ids) hs s locs (HE_value HV_trap)
   | pr_call_trap3:
     forall hs s locs id ids i,
-      hs !! id = Some (Some (HV_wov (WOV_funcref (Mk_funcidx i)))) ->
+      hs !! id = Some (HV_wov (WOV_funcref (Mk_funcidx i))) ->
       s.(s_funcs) !! i = None ->
       pure_reduce hs s locs (HE_call id ids) hs s locs (HE_value HV_trap)  
   | pr_call_trap4:
     forall hs s locs id ids,
-      list_extra.those2 (map (fun id => hs !! id) ids) = None ->
+      list_extra.those (map (fun id => hs !! id) ids) = None ->
       pure_reduce hs s locs (HE_call id ids) hs s locs (HE_value HV_trap)
   | pr_call_wasm_trap1:
     forall hs s locs id ids i cl j tf vts bes vars tn tm,
-      hs !! id = Some (Some (HV_wov (WOV_funcref (Mk_funcidx i)))) ->
+      hs !! id = Some (HV_wov (WOV_funcref (Mk_funcidx i))) ->
       s.(s_funcs) !! i = Some cl ->
       cl = FC_func_native j tf vts bes ->
       tf = Tf tn tm ->
-      list_extra.those2 (map (fun id => hs !! id) ids) = Some vars ->
+      list_extra.those (map (fun id => hs !! id) ids) = Some vars ->
       list_host_value_to_wasm vars = None ->
       pure_reduce hs s locs (HE_call id ids) hs s locs (HE_value HV_trap)  
   | pr_call_wasm_trap2:
     forall hs s locs id ids i cl j tf vts bes vars tn tm vs,
-      hs !! id = Some (Some (HV_wov (WOV_funcref (Mk_funcidx i)))) ->
+      hs !! id = Some (HV_wov (WOV_funcref (Mk_funcidx i))) ->
       s.(s_funcs) !! i = Some cl ->
       cl = FC_func_native j tf vts bes ->
       tf = Tf tn tm ->
-      list_extra.those2 (map (fun id => hs !! id) ids) = Some vars ->
+      list_extra.those (map (fun id => hs !! id) ids) = Some vars ->
       list_host_value_to_wasm vars = Some vs ->
       tn <> map typeof vs ->
       pure_reduce hs s locs (HE_call id ids) hs s locs (HE_value HV_trap)  
   | pr_call_host:
     forall hs s ids cl id i n e tf tn tm vars vs locs,
-      hs !! id = Some (Some (HV_wov (WOV_funcref (Mk_funcidx i)))) ->
+      hs !! id = Some (HV_wov (WOV_funcref (Mk_funcidx i))) ->
       s.(s_funcs) !! i = Some cl ->
       cl = FC_func_host tf n e ->
       tf = Tf tn tm ->
-      list_extra.those2 (map (fun id => hs !! id) ids) = Some vars ->
+      list_extra.those (map (fun id => hs !! id) ids) = Some vars ->
       list_host_value_to_wasm vars = Some vs -> (* TODO: change this to explicit casts, then add a trap case. *)
       tn = map typeof vs ->
       pure_reduce hs s locs (HE_call id ids) hs s locs (HE_wasm_frame ((v_to_e_list vs) ++ [::AI_invoke i]))
@@ -335,16 +331,16 @@ Inductive pure_reduce : host_state -> store_record -> list host_value -> host_ex
       pure_reduce hs s locs (HE_wasm_table_create len) hs s' locs (HE_value (HV_wov (WOV_tableref (Mk_tableidx n))))
   | pr_table_set:
     forall hs s locs idt n id v tn tab tab' s' fn,
-      hs !! idt = Some (Some (HV_wov (WOV_tableref (Mk_tableidx tn)))) ->
+      hs !! idt = Some (HV_wov (WOV_tableref (Mk_tableidx tn))) ->
       s.(s_tables) !! tn = Some tab ->
-      hs !! id = Some (Some v) ->
+      hs !! id = Some v ->
       v = HV_wov (WOV_funcref (Mk_funcidx fn)) ->
       tab' = {|table_data := list_insert n (Some fn) tab.(table_data); table_max_opt := tab.(table_max_opt) |} ->
       s' = {|s_funcs := s.(s_funcs); s_tables := list_insert tn tab' s.(s_tables); s_mems := s.(s_mems); s_globals := s.(s_globals) |} ->
       pure_reduce hs s locs (HE_wasm_table_set idt (N_of_nat n) id) hs s' locs (HE_value v)
   | pr_table_get:
     forall hs s locs idt n tn tab fn,
-      hs !! idt = Some (Some (HV_wov (WOV_tableref (Mk_tableidx tn)))) ->
+      hs !! idt = Some (HV_wov (WOV_tableref (Mk_tableidx tn))) ->
       s.(s_tables) !! tn = Some tab ->
       tab.(table_data) !! n = Some (Some fn) ->
       pure_reduce hs s locs (HE_wasm_table_get idt (N_of_nat n)) hs s locs (HE_value (HV_wov (WOV_funcref (Mk_funcidx fn))))
@@ -355,22 +351,22 @@ Inductive pure_reduce : host_state -> store_record -> list host_value -> host_ex
       pure_reduce hs s locs (HE_wasm_memory_create sz sz_lim) hs s' locs (HE_value (HV_wov (WOV_memoryref (Mk_memidx n))))
   | pr_memory_set:
     forall hs s locs idm n id md' mn m m' s' b,
-      hs !! idm = Some (Some (HV_wov (WOV_memoryref (Mk_memidx mn)))) ->
+      hs !! idm = Some (HV_wov (WOV_memoryref (Mk_memidx mn))) ->
       s.(s_mems) !! mn = Some m ->
-      hs !! id = Some (Some (HV_byte b)) ->
+      hs !! id = Some (HV_byte b) ->
       memory_list.mem_update n b m.(mem_data) = Some md' ->
       m' = {|mem_data := md'; mem_max_opt := m.(mem_max_opt) |} ->
       s' = {|s_funcs := s.(s_funcs); s_tables := s.(s_tables); s_mems := list_insert mn m' s.(s_mems); s_globals := s.(s_globals) |} ->
       pure_reduce hs s locs (HE_wasm_memory_set idm n id) hs s' locs (HE_value (HV_byte b))
   | pr_memory_get:
     forall hs s locs idm n b m mn,
-      hs !! idm = Some (Some (HV_wov (WOV_memoryref (Mk_memidx mn)))) ->
+      hs !! idm = Some (HV_wov (WOV_memoryref (Mk_memidx mn))) ->
       s.(s_mems) !! mn = Some m ->
       memory_list.mem_lookup n m.(mem_data) = Some b ->
       pure_reduce hs s locs (HE_wasm_memory_get idm n) hs s locs (HE_value (HV_byte b))
   | pr_memory_grow:
     forall hs s s' locs idm n m m' mn,
-      hs !! idm = Some (Some (HV_wov (WOV_memoryref (Mk_memidx mn)))) ->
+      hs !! idm = Some (HV_wov (WOV_memoryref (Mk_memidx mn))) ->
       s.(s_mems) !! mn = Some m ->
       mem_grow m n = Some m' ->
       s' = {|s_funcs := s.(s_funcs); s_tables := s.(s_tables); s_mems := list_insert mn m' s.(s_mems); s_globals := s.(s_globals) |} ->
@@ -382,8 +378,8 @@ Inductive pure_reduce : host_state -> store_record -> list host_value -> host_ex
       pure_reduce hs s locs (HE_wasm_global_create g) hs s' locs (HE_value (HV_wov (WOV_globalref (Mk_globalidx n))))
   | pr_global_set:
     forall hs s locs gn idg id s' v g g',
-      hs !! id = Some (Some (HV_wasm_value v)) ->
-      hs !! idg = Some (Some (HV_wov (WOV_globalref (Mk_globalidx gn)))) ->
+      hs !! id = Some (HV_wasm_value v) ->
+      hs !! idg = Some (HV_wov (WOV_globalref (Mk_globalidx gn))) ->
       s.(s_globals) !! gn = Some g ->
       g.(g_mut) = MUT_mut ->
       typeof v = typeof (g.(g_val)) ->
@@ -392,22 +388,22 @@ Inductive pure_reduce : host_state -> store_record -> list host_value -> host_ex
       pure_reduce hs s locs (HE_wasm_global_set idg id) hs s' locs (HE_value (HV_wasm_value v))
   | pr_global_get:
     forall hs s locs idg g gn v,
-      hs !! idg = Some (Some (HV_wov (WOV_globalref (Mk_globalidx gn)))) ->
+      hs !! idg = Some (HV_wov (WOV_globalref (Mk_globalidx gn))) ->
       g.(g_val) = v ->
       pure_reduce hs s locs (HE_wasm_global_get idg) hs s locs (HE_value (HV_wasm_value v))
   (* wasm module expr *)
    (* TODO: add this back after specifying the concrete host *)
  (* | pr_compile:
     forall hs s locs id mo hvl hbytes,
-      hs !! id = Some (Some (HV_list hvl)) ->
+      hs !! id = Some (HV_list hvl) ->
       to_bytelist hvl = Some hbytes ->
       run_parse_module (map byte_of_compcert_byte hbytes) = Some mo -> (* Check: is this correct? *)
       pure_reduce hs s locs (HE_compile id) hs s locs (HE_value (HV_module mo))*)
   (* TODO: replace the proxy *)
   | pr_instantiate:
     forall hs s locs idm idr mo r rec,
-      hs !! idm = Some (Some (HV_module mo)) ->
-      hs !! idr = Some (Some (HV_record r)) ->
+      hs !! idm = Some (HV_module mo) ->
+      hs !! idr = Some (HV_record r) ->
       pure_reduce hs s locs (HE_instantiate idm idr) hs s locs rec
   (* miscellaneous *)
   | pr_seq_const:
@@ -421,7 +417,7 @@ Inductive pure_reduce : host_state -> store_record -> list host_value -> host_ex
       pure_reduce hs s locs (HE_wasm_frame ([::AI_trap])) hs s locs (HE_value (HV_trap))
   | pr_host_return:
     forall hs s locsf locs ids e vs tn,
-      list_extra.those2 (map (fun id => hs !! id) ids) = Some vs ->
+      list_extra.those (map (fun id => hs !! id) ids) = Some vs ->
       pure_reduce hs s locsf (HE_host_frame tn locs (HE_seq (HE_return ids) e)) hs s locsf (HE_value (HV_list vs))
 
 (* TODO: needs all the host_expr reduction steps: compile, instantiate, etc. *)
@@ -491,7 +487,7 @@ with wasm_reduce : host_state -> store_record -> datatypes_iris.frame -> list ad
   | wr_host_return :
     (* TODO: check *)
     forall hs s f ts vs ids vs' vs'',
-    list_extra.those2 (map (fun id => hs !! id) ids) = Some vs' ->
+    list_extra.those (map (fun id => hs !! id) ids) = Some vs' ->
     Some vs'' = list_extra.those (List.map (fun x => match x with | HV_wasm_value v => Some v | _ => None end) vs') ->
     wasm_reduce hs s f [::AI_host_frame ts vs (HE_return ids)] hs s f (v_to_e_list vs'')
 (*  
